maps.v
@@ -1,0 +1,30 @@
+Set Warnings "-notation-overridden,-parsing,-deprecated-hint-without-locality".
+From Coq Require Import Strings.String.
+From Coq Require Import Strings.String.
+From Coq Require Import Lists.List.
+
+Notation "x :: l" := (cons x l)
+                     (at level 60, right associativity).
+Notation "[ ]" := nil.
+Notation "[ x ; .. ; y ]" := (cons x .. (cons y nil) ..).
+
+Definition total_map (A : Type) := string -> A.
+Definition t_empty {A : Type} (v : A) : total_map A :=
+  (fun _ => v).
+Definition t_update {A : Type} (m : total_map A)
+                    (x : string) (v : A) :=
+  fun x' => if String.eqb x x' then v else m x'.
+Notation "'_' '!->' v" := (t_empty v)
+  (at level 100, right associativity).
+Notation "x '!->' v ';' m" := (t_update m x v)
+                              (at level 100, v at next level, right associativity).
+Definition partial_map (A : Type) := total_map (option A).
+Definition empty {A : Type} : partial_map A :=
+  t_empty None.
+Definition update {A : Type} (m : partial_map A)
+           (x : string) (v : A) :=
+  (x !-> Some v ; m).
+Notation "x '|->' v ';' m" := (update m x v)
+  (at level 100, v at next level, right associativity).
+Notation "x '|->' v" := (update empty x v)
+  (at level 100).
